src/ReactorModel/Determinism/InstantaneousStep.lean
@@ -7,57 +7,30 @@ namespace Instantaneous
 namespace Step
 
 variable [Indexable α] {s₁ s₂ : State α} in section
-
-theorem rcn_not_mem_progress (e : s₁ ⇓ᵢ s₂) : e.rcn ∉ s₁.progress := 
-  sorry -- e.allows.unprocessed
-
-theorem preserves_tag (e : s₁ ⇓ᵢ s₂) : s₁.tag = s₂.tag := 
-  sorry -- e.exec.preserves_tag
   
-theorem mem_progress_iff :
-  (e : s₁ ⇓ᵢ s₂) → (rcn' ∈ s₂.progress ↔ rcn' = e.rcn ∨ rcn' ∈ s₁.progress) := by
-  intro h
-  constructor
-  case mp =>
-    intro ho
-    by_cases hc : rcn' = h.rcn
-    case pos => exact .inl hc
-    case neg => sorry
-      -- rw [State.progress, h.exec.ctx_adds_rcn, ←rcn] at ho
-      -- simp [Context.mem_record_progress_iff _ _ _ |>.mp ho]
-  case mpr =>
-    intro ho
-    by_cases hc : rcn' = h.rcn
-    case pos =>
-      simp [hc]
-      sorry
-      -- exact Context.mem_record_progress_iff _ _ _ |>.mpr (.inl rfl)
-    case neg =>
-      sorry
-      -- simp [State.progress, h.exec.ctx_adds_rcn, Context.mem_record_progress_iff _ _ _ |>.mpr (.inr $ ho.resolve_left hc)]
+theorem mem_progress_iff : (e : s₁ ⇓ᵢ s₂) → (rcn' ∈ s₂.progress ↔ rcn' = e.rcn ∨ rcn' ∈ s₁.progress)
+  | skip .. | exec .. => s₁.mem_record_progress_iff _ _
 
 -- Corollary of `InstStep.mem_progress_iff`.
-theorem not_mem_progress :
-  (e : s₁ ⇓ᵢ s₂) → (rcn' ≠ e.rcn) → rcn' ∉ s₁.progress → rcn' ∉ s₂.progress := 
-  sorry -- λ h hn hm => (mt h.mem_progress.mp) $ not_or.mpr ⟨hn, hm⟩
+theorem progress_monotonic (e : s₁ ⇓ᵢ s₂) (h : rcn' ∈ s₁.progress) : rcn' ∈ s₂.progress := 
+  e.mem_progress_iff.mpr $ .inr h
 
--- Corollary of `InstStep.mem_progress`.
-theorem monotonic_progress : (s₁ ⇓ᵢ s₂) → rcn' ∈ s₁.progress → rcn' ∈ s₂.progress := 
-  sorry -- (·.mem_progress_iff.mpr $ .inr ·)
-
--- Corollary of `InstStep.mem_progress`.
+-- Corollary of `InstStep.mem_progress_iff`.
 theorem rcn_mem_progress : (e : s₁ ⇓ᵢ s₂) → e.rcn ∈ s₂.progress := 
   (·.mem_progress_iff.mpr $ .inl rfl)
 
-theorem not_Closed (e : s₁ ⇓ᵢ s₂) : ¬s₁.Closed := by
-  intro c
-  have h := c ▸ e.allows_rcn.unprocessed
-  simp [Partial.mem_iff] at h 
-  sorry -- have := h e.allows.mem.choose
-  -- contradiction 
+theorem rcn_not_mem_progress (e : s₁ ⇓ᵢ s₂) : e.rcn ∉ s₁.progress := 
+  e.allows_rcn.unprocessed
 
-theorem equiv : (s₁ ⇓ᵢ s₂) → s₁.rtr ≈ s₂.rtr :=
-  sorry
+theorem not_Closed (e : s₁ ⇓ᵢ s₂) : ¬s₁.Closed :=
+  (· ▸ e.allows_rcn.unprocessed $ e.allows_rcn.mem)
+
+theorem preserves_tag : (s₁ ⇓ᵢ s₂) → s₁.tag = s₂.tag
+  | skip .. | exec .. => rfl
+
+theorem equiv : (s₁ ⇓ᵢ s₂) → s₁.rtr ≈ s₂.rtr
+  | skip .. => .refl
+  | exec .. => s₁.exec_equiv _
 
 theorem deterministic (e₁ : s ⇓ᵢ s₁) (e₂ : s ⇓ᵢ s₂) (h : e₁.rcn = e₂.rcn) : s₁ = s₂ := by
   cases e₁ <;> cases e₂
@@ -71,7 +44,7 @@ theorem progress_eq : (e : s₁ ⇓ᵢ s₂) → s₂.progress = s₁.progress.i
 
 theorem seq_wellordered (e₁ : s₁ ⇓ᵢ s₂) (e₂ : s₂ ⇓ᵢ s₃) : e₂.rcn ≮[s₁.rtr] e₁.rcn := by
   by_contra d
-  exact e₂.allows_rcn.unprocessed $ e₁.monotonic_progress $ e₁.allows_rcn.deps d
+  exact e₂.allows_rcn.unprocessed $ e₁.progress_monotonic $ e₁.allows_rcn.deps d
 
 theorem seq_rcn_ne (e₁ : s₁ ⇓ᵢ s₂) (e₂ : s₂ ⇓ᵢ s₃) : e₁.rcn ≠ e₂.rcn := by
   by_contra he
@@ -85,7 +58,7 @@ theorem prepend_indep' (e₁ : s₁ ⇓ᵢ s₂) (e₂ : s₂ ⇓ᵢ s₃) (h : 
     ∃ (s₂' : _) (s₃' : _) (e₁' : s₁ ⇓ᵢ s₂') (e₂' : s₂' ⇓ᵢ s₃'), 
       (e₁'.rcn = e₂.rcn) ∧ (e₂'.rcn = e₁.rcn) ∧ (s₃' = s₃) := by
   have hi : _ ≮[_]≯ _ := { not_eq := e₁.seq_rcn_ne e₂, left := h, right := e₁.seq_wellordered e₂ }
-  cases e₁ <;> cases e₂ <;> simp [rcn] at hi
+  cases e₁ <;> cases e₂ <;> simp [rcn] at hi  
   case skip.skip ha₁ ht₁ rcn₂ ha₂ ht₂ =>
     have ha₁' := State.record_indep_allows_iff hi.symm |>.mp ha₁
     have ha₂' := State.record_indep_allows_iff hi |>.mpr ha₂
@@ -112,7 +85,7 @@ theorem prepend_indep' (e₁ : s₁ ⇓ᵢ s₂) (e₂ : s₂ ⇓ᵢ s₃) (h : 
     have ht₁' := State.exec_record_indep_triggers_iff hi |>.mp ht₁
     have ht₂' := State.exec_record_indep_triggers_iff hi.symm |>.mpr ht₂
     refine ⟨_, _, Step.exec ha₂' ht₂', Step.exec ha₁' ht₁', rfl, rfl, ?_⟩
-    simp [rcn, State.record_exec_comm, State.record_comm, State.exec_indep_comm hi.symm]
+    simp [rcn, State.record_exec_comm, State.record_comm, State.exec_indep_comm hi]
 
 theorem prepend_indep (e₁ : s₁ ⇓ᵢ s₂) (e₂ : s₂ ⇓ᵢ s₃) (h : e₁.rcn ≮[s₁.rtr] e₂.rcn) :
     ∃ (s₂' : _) (e₁' : s₁ ⇓ᵢ s₂') (e₂' : s₂' ⇓ᵢ s₃), (e₁'.rcn = e₂.rcn) ∧ (e₂'.rcn = e₁.rcn) := by
